nettoyage

code/coq/det.v
@@ -60,257 +60,56 @@ Fixpoint has_cut l :=
 
 Fixpoint all_has_cut (l: seq (seq pred)) :=
   match l with
-  | [::] => False
-  | [::x] => has_cut x
+  | [::] => True
   | [::x&xs] =>
     has_cut x /\ all_has_cut xs
   end.
 
 Definition all_have_cut (p: bodiesT) :=
-  forall f, p f <> [::] /\ all_has_cut (p f).
+  forall f, all_has_cut (p f).
 
-(* Lemma next_alt_help prog p n:
-forall a befs aft l0 r,
-prog p = [::] ->
-  next_alt
-([seq [seq Goal x a  | x <- b] ++
-rcons (not_alt_goal befs) (Goal (call p) [::]) ++ aft
- | b <- l0] ++ a) (run prog n) = r ->
-  exists n', next_alt a (run prog n') = r.
+Lemma all_goals_with_cut prog n r:
+  forall g gs tl, all_have_cut prog ->
+    all_has_cut (g :: gs) ->
+      (* in all goal (g::gs) we have a bang and each of them has no cut-alternatives,
+            therefore, 
+              -if a goal g' in (g::gs) succeeds, we have
+                the same result as running the goal g' alone (the alternative being rejected)
+              -otherwise, if all goals fails, the lemma is trivial
+            
+       *)
+      run prog n (not_alt_goal (g ++ tl)) 
+        [seq [seq Goal x [::]  | x <- b] ++ not_alt_goal tl | b <- gs] = r ->
+      exists g n', n' <= n /\ run prog n' (not_alt_goal g) [::] = r.
 Proof.
-Admitted. *)
-
-Lemma cut_does_cut prog n: forall gs befs aft l0 r,
-   run prog n (not_alt_goal (rcons (gs ++ befs) cut ++ aft))
-    [seq [seq Goal x [::]  | x <- b] ++ not_alt_goal (rcons befs cut ++ aft) | b <- l0] = r -> 
-        exists gs', run prog n (not_alt_goal (rcons (gs' ++ befs) cut ++ aft)) [::] = r.
-Proof.
-  induction n.
-  exists [::]; simpl; auto.
-  simpl.
-  destruct gs as [|g gs]; simpl.
-  1:{
-      destruct befs as [|bef befs]; simpl.
-      now exists ([::]).
-      destruct bef as [|p]; [exists [::]; auto|].
-      destruct (prog p) eqn:PP.
-      1:{
-        move => aft [|G GS]; simpl.
-        1:{
-          inversion 1; exists (call p :: [::]); simpl; rewrite PP; auto.
-        }
-        replace  ([seq Goal x [::]  | x <- G] ++ Goal (call p) [::] :: not_alt_goal (rcons befs cut ++ aft)) with
-                (not_alt_goal (rcons (rcons G (call p) ++ befs) cut ++ aft)).
-        2:{
-            rewrite rcons_cat.
-            rewrite <-cats1.
-            do 2 rewrite <-catA.
-            rewrite <-not_alt_goal_app; f_equal.
-          }
+  destruct r as [s|].
+  2:{ intros. exists [::], 0; auto. }
+  (* here r is Some s*)
+  induction n; [by []|].
+  destruct g as [|G GTL].
+    - move=> ??? [] //.
+    - (* here g is not empty: it is the list [G|GTL] *)
+      move=> gs tl ACP ACG.
+      destruct G as [|p].
+      now intros; exists (GTL++tl), n.
+      - (* here G is a call of a predicate p *)
+        assert (all_has_cut (GTL :: gs)) by auto.
+        clear ACG.
+        destruct (prog p) as [|sol sols] eqn:PP.
+        + (*here no solution for prog p*)
+          simpl; rewrite PP.
+          destruct gs; [by[]|].
+          (*here gs is non empty*)
+          simpl.
           intros.
+          destruct H as [].
+          rewrite not_alt_goal_app in H0.
+          specialize (IHn l gs tl ACP H1 H0) as [?[?[]]].
+          exists x, x0; split; auto.
+        + (*here prog p has some solutions (sol::sols)*)
+          simpl.
+          rewrite PP.
 
-          (* apply failing_goal in H.
-          specialize (IHn _ _ _ _ _ H). *)
-          admit.
-      }
-      admit.
-  }
-  admit.
-          
-Admitted.
-
-Lemma func_after_bang prog:
-  forall bef aft,
-    functional_goal prog aft -> 
-      functional_goal prog (rcons bef cut ++ aft).
-Proof.
-  intros.
-  intros ?.
-  revert bef.
-  induction n; auto.
-  simpl.
-  destruct bef as [|bef befs]; simpl.
-  1:{
-      intros.
-      eapply H.
-      apply H0.
-   }
-   destruct bef.
-   1:{
-    apply IHn.
-   }
-   destruct (prog p) eqn:?; auto.
-   intros r.
-   rewrite cats0.
-   rewrite not_alt_goal_app.
-   rewrite catA.
-   rewrite <-rcons_cat.
-   intros.
-   eapply cut_does_cut in H0 as[].
-   epose proof (IHn _ _ H0); auto.
-Qed.
-
-(* Lemma xxxxx gs GS:
-  [seq [seq Goal x [::]  | x <- b] ++ not_alt_goal gs  | b <- [seq rcons x cut  | x <- GS]] =
-  [seq (not_alt_goal (b++gs)) | b <- [seq rcons x cut  | x <- GS]].
-      f_equal.
-      apply functional_extensionality; intros. *)
-
-Lemma map_app {T:Type} {S:Type}:
-  forall (f: T -> S) l1 l2, [seq f x | x <- l1] ++ [seq f x | x <- l2] = [seq f x | x <- l1 ++ l2].
-  Admitted.
-
-(* Lemma pop_goal prog r n:
-  forall g1 a,
-    forall k, run prog k g1 a = Some r
-    -> forall g2, run prog (n+k) (g1 ++ g2) a = Some r.  *)
-
-  (* TODO: if we have bang wherever, then exists one of them
-  producing the same result *)
-
-  (* 
-  
-  run prog n (not_alt_goal (l ++ gs))
-[seq [seq Goal x [::]  | x <- b] ++ not_alt_goal gs
- | b <- l0] = r
-   *)
-
-
-Lemma all_have_cut'' prog n: forall l l0 ls gs r l1,
-  all_has_cut l1 ->
-    all_has_cut (l::l0)->
-      let T:=[seq [seq Goal x0 [::]  | x0 <- b] ++ not_alt_goal gs  | b <- l1] in
-  run prog n ([seq Goal x T  | x <- l] ++ not_alt_goal (ls ++ gs))
-      ([seq [seq Goal x T  | x <- b] ++ not_alt_goal (ls ++ gs)  | b <- l0] ++ T) =
-r -> exists n', 
-  n' <= n /\
-    run prog n' (not_alt_goal (l ++ gs)) 
-      [seq [seq Goal x [::]  | x <- b] ++ not_alt_goal gs  | b <- l0] = r.
-Proof.
-  simpl; intros.
-  destruct r.
-  2:{ exists 0; auto. }
-Admitted.
-
-Lemma all_have_cut_general prog n:
-all_have_cut prog ->
-    forall gs tl (ll:seq (seq goal)) r, all_has_cut gs ->
-      next_alt [seq [seq Goal x ll | x <- b] ++ tl | b <- gs] (run prog n) = Some r ->
-        exists g n', n' <= n /\ run prog n' ([seq Goal x ll | x <- g] ++ tl) ll = Some r. (*g ∈ gs*)
-Proof.
-
-  (* enough (forall n tl (ll:seq (seq goal)) r, all_has_cut gs ->
-      next_alt [seq not_alt_goal (b++tl) | b <- gs] (run prog n) = Some r ->
-        exists g n', n' <= n /\ run prog n' ([seq Goal x [::] | x <- g]) [::] = Some r (*g ∈ gs*)) by admit.
-  intro. *)
-  intros HProg.
-  induction n; move=> [] // g gs.
-  destruct g.
-  intros; simpl in H; destruct gs; try easy.
-  destruct p.
-  simpl; move=> tl ll r _ H. exists (g), n; constructor; auto.
-
-    
-  destruct (prog p) eqn:PP.
-  simpl; rewrite PP.
-  destruct gs; try by [].
-  move=> tl ll r [C1 C2].
-  simpl.
-  intros.
-  specialize (IHn (l::gs) tl ll r C2).
-
-  simpl in IHn.
-  apply IHn in H as (?&?&?&?).
-  exists x, x0; auto.
-
-  move=> tl ll r H.
-  simpl.
-  rewrite PP.
-  assert (all_has_cut (g::gs)).
-  auto.
-  pose (
-    [seq Goal x [seq [seq Goal x0 ll  | x0 <- b] ++ tl | b <- gs] | x <- l] 
-      ++ [seq Goal x ll  | x <- l] ++ tl) as T.
-  fold T.
-
-  (* rewrite <-map_app. *)
-  (* epose proof (IHn _ ([seq Goal x ll  | x <- l] ++ tl) 
-    ([seq [seq Goal x0 ll  | x0 <- b] ++ tl  | b <- gs]) r H0). *)
-  epose proof (IHn _ _
-    _ r H0).
-  simpl in H1.
-  Unshelve.
-  3:{ apply [seq [seq Goal x0 ll  | x0 <- b] ++ tl  | b <- gs]. }
-  Admitted.
-  
-
-
-
-Lemma all_have_cut' prog n:
-    forall gs tl (ll:seq (seq goal)) r, all_has_cut gs ->
-      next_alt [seq [seq Goal x [::] | x <- b] ++ not_alt_goal tl | b <- gs] (run prog n) = Some r ->
-        exists g n', n' <= n /\ run prog n' ([seq Goal x [::] | x <- g]) [::] = Some r. (*g ∈ gs*)
-Proof.
-
-  (* enough (forall n tl (ll:seq (seq goal)) r, all_has_cut gs ->
-      next_alt [seq not_alt_goal (b++tl) | b <- gs] (run prog n) = Some r ->
-        exists g n', n' <= n /\ run prog n' ([seq Goal x [::] | x <- g]) [::] = Some r (*g ∈ gs*)) by admit.
-  intro. *)
-
-  induction n; move=> [] // g gs.
-  destruct g.
-  intros; simpl in H; destruct gs; try easy.
-  destruct p.
-  simpl; move=> tl _ r _; rewrite map_app; exists (g++tl), n; auto.
-  destruct (prog p) eqn:PP.
-  simpl; rewrite PP.
-  destruct gs; try by [].
-  move=> tl _ r [C1 C2].
-  simpl.
-  intros.
-  specialize (IHn (l::gs) tl [::] r C2).
-
-  simpl in IHn.
-  apply IHn in H as (?&?&?&?).
-  exists x, x0; auto.
-
-  move=> tl _ r H.
-  simpl.
-  rewrite PP.
-  rewrite map_app.
-  simpl.
-  epose proof (IHn _ tl _ r H).
-  simpl in H0.
-
-
-  simpl in H0.
-  (* apply pumping1 in H0. *)
- 
-
-
-  (* induction eapply IHn; apply H0.
-  destruct (prog p) as [|sol sols] eqn:PP; auto.
-  rewrite cats0.
-  destruct r; auto.
-  intro.
-  unfold not_alt_goal in IHn.
-  specialize (H p) as [? ALL_CUT].
-  rewrite PP in ALL_CUT.
-  pose proof (all_have_cut' _ _ _ _ [::] _ ALL_CUT H0) as [gg[nn [leq HH]]].
-  apply (pumping_leq _ _ _ _ _ _ leq) in HH.
-  now pose proof (IHn _ _ HH).
-Qed. gs as [|g gs]; [by []|]; simpl in *.
-  destruct gs; simpl in *.
-  intros.
-  exists (g ++ tl); simpl.
-  rewrite map_app in H0.
-  exists n; auto.
-  ------
-  destruct H as [CUT_G CUT_GS].
-  specialize (IHgs CUT_GS).
-  intros.
-  repeat rewrite map_app in H.
-  specialize (IHgs (g ++ tl) n ll r). *)
 
 Admitted.
 
@@ -323,92 +122,44 @@ Proof.
   simpl.
   destruct g as [|g gs]; simpl; auto.
   destruct g as [|p].
-
-
-
-Admitted.
-
-  (* intros; eapply IHn; apply H0.
-  destruct (prog p) as [|sol sols] eqn:PP; auto.
+  apply IHn.
+  destruct (prog p) eqn:?.
+  auto.
   rewrite cats0.
+  rewrite not_alt_goal_app.
+  intro.
   destruct r; auto.
-  intro.
-  unfold not_alt_goal in IHn.
-  specialize (H p) as [? ALL_CUT].
-  rewrite PP in ALL_CUT.
-  pose proof (all_have_cut' _ _ _ _ [::] _ ALL_CUT H0) as [gg[nn [leq HH]]].
-  apply (pumping_leq _ _ _ _ _ _ leq) in HH.
-  now pose proof (IHn _ _ HH).
-Qed. *)
+  pose proof (H p) as Hp.
+  rewrite Heql in Hp.
+  apply all_goals_with_cut in H0 as [?[?[]]]; auto.
+  epose proof (pumping_leq _ _ _ _ _ _ H0 H1).
+  eapply IHn.
+  apply H2.
+Qed.
 
-Fixpoint In {A:Type} (a:A) (l:list A) : Prop :=
-    match l with
-      | nil => False
-      | b :: m => b = a \/ In a m
-    end.
-
-(* Lemma blah prog n l:
-  forall G GS gs,
-    run (tail_cut_all prog) n (not_alt_goal (rcons G cut ++ gs))
-[seq not_alt_goal (b ++ gs)  | b <- [seq rcons x cut  | x <- GS]] = Some l ->
-    exists G', run (tail_cut_all prog) n (not_alt_goal G') [::] = Some l.
-Proof.
-  elim: n=> // n IH.
-  intro.
-  destruct (rcons G cut) as [|G' GS'] eqn:RC.
-  destruct (rcons_non_empty _ _ RC).
-  destruct G'.
-  1:{ simpl.
-    intros.
-    destruct G; inversion RC; subst; clear RC.
-    2:{
-      specialize (IH G [::] gs).
-      simpl in IH.
-      specialize (IH H) as [].
-      exists (cut :: rcons G cut ++ gs); simpl; auto.
-    }
-    simpl in H.
-    exists (cut :: gs).
-    now simpl.
-  }
-  intros GS gs.
-  simpl.
-  unfold tail_cut_all.
-  destruct (prog p) eqn:?; simpl.
-  destruct GS.
-  by [].
-  simpl.
-  fold_tail_cut_all prog.
-  
-  intros.
-  specialize (IH _ _ _ H) as [].
-  exists (cut :: x); auto.
-
-  fold_tail_cut_all prog.
-  intros.
-Admitted. *)
-
-
-(* Lemma all_have_cut_tail_cut_all:
+Lemma all_have_cut_tail_cut_all:
   forall p, all_have_cut(tail_cut_all p).
 Proof.
   unfold tail_cut_all.
   intros ??.
   destruct (p f); simpl; auto.
-  2:{ split; auto. destruct l0. inversion 1.
-      simpl. }
   split.
-  intros ?.
-  destruct (p f); simpl in H.
-  destruct (rcons_non_empty _ _ H).
-  simpl.
-  induction f. *)
+  induction l; simpl; auto.
+  destruct a; auto.
+  induction l0; simpl; auto.
+  constructor; auto.
+  induction a; simpl; auto.
+  destruct a; auto.
+Qed.
 
 Lemma functional_tail_cut_all:
   forall p, functional_prog (tail_cut_all p).
 Proof.
-  (* intros ??.
-  induction n; auto. *)
+  intro.
+  now pose proof (functional_all_with_cut (tail_cut_all p) (all_have_cut_tail_cut_all p)).
+Qed.
+  (*Old incomplete proof without functional_all_with_cut *)
+  (* simpl.
   intros prog n r.
   elim: n => /=.
   - move => _ ->; auto.
@@ -436,9 +187,9 @@ Proof.
       apply functional_extensionality; intros.
       now rewrite not_alt_goal_app.
       rewrite H' in H.
-      clear H'.
+      clear H'. *)
 
-Admitted.
+(* Admitted. *)
 
 
 
